\documentclass{article}
\usepackage[utf8]{inputenc}

\title{MLT Homework 11}
% \author{Ana Borovac \\ Jonas Haslbeck \\ Bas Haver} % I'll be coming back :-)
\author{Ana Borovac  \\ Bas Haver}

\usepackage{natbib}
\usepackage{graphicx}
\usepackage{subcaption}

\usepackage{amsmath}
\usepackage{amsfonts}
\usepackage{amssymb}
\usepackage{bbm}
\usepackage{mathtools}

\usepackage{url}

\DeclarePairedDelimiter\ceil{\lceil}{\rceil}
\DeclarePairedDelimiter\floor{\lfloor}{\rfloor}

\newcommand{\Hy}{\mathcal{H}}
\newcommand{\VC}{\text{VCdim}}

\newcounter{counterquestion}
\newenvironment{question}[1]
{
\stepcounter{counterquestion}
\section*{Question \thecounterquestion}
\emph{#1} 
} 
{
}

\newcounter{countersubquestion}[counterquestion]
\newenvironment{subquestion}[1]
{
\stepcounter{countersubquestion}
\subsection*{Subquestion \thecounterquestion .\thecountersubquestion}
\emph{#1} 
} 
{
}

\newenvironment{solution}
{
\subsubsection*{Solution}
} 
{
}


\begin{document}

\maketitle

% 1st question
\begin{question}{}
\end{question}

% 2nd question
\begin{question}{}
\end{question}

% 3rd question
\begin{question}{Determine whether the following functions are exp-concave, and to what degree.}

\begin{subquestion}{$x \mapsto (x - y)^2$ on $x, y \in [-Y, Y]$ First consider a fixed $y$ and then determine the worst-case over all $y \in [-Y, Y]$.}
\begin{solution}
Let's recall the definition of $\alpha$-exp-concave function: A function $f$ is $\alpha$-exp-concave if $x \mapsto e^{-\alpha f(x)}$ is concave.

In our case we get:
\begin{align*}
x \mapsto e^{-\alpha (x - y)^2} \quad & \Rightarrow \quad g(x) = e^{-\alpha (x - y)^2} \\
& \Rightarrow \quad g'(x) = -2 \alpha (x - y)e^{-\alpha (x - y)^2} \\
& \Rightarrow \quad g''(x) = -2 \alpha e^{-\alpha (x - y)^2} + 4 \alpha^2 (x - y)^2 e^{-\alpha (x - y)^2} \\
\end{align*}
%
If $g$ is concave then $g''(x) \leq 0$ for $\forall x$.
\begin{align*}
-2 \alpha e^{-\alpha (x - y)^2} + 4 \alpha^2 (x - y)^2 e^{-\alpha (x - y)^2} & \leq 0 \\
\underbrace{e^{-\alpha (x - y)^2}}_{\geq 0} (-2 \alpha + 4 \alpha^2 (x - y)^2) & \leq 0 \\
2  \alpha ( - 1+ 2 \alpha (x - y)^2) & \leq 0 \\
 - 1+ 2 \alpha (x - y)^2 & \leq 0 \\
\alpha & \leq \frac{1}{2 (x - y)^2} \\
\end{align*}

If we want to inequality to hold for $\forall x$ we need to observe when the fraction on the right is the smallest. So, when does $(x - y)^2$ reach maximum? It depands on $y$, but it is obvious that it is reached when $x$ is $Y$ or $-Y$, so:
\[
\alpha = \frac{1}{2 \max \{ (Y - y)^2, (-Y - y)^2 \}}
\]

In the worst case the difference between $x$ and $y$ is $2Y$. From that it follows:
\[
\alpha = \frac{1}{8 Y^2}
\]
\end{solution}
\end{subquestion}

\begin{subquestion}{$x \mapsto |x|^p$ on $x \in [-1, 1]$ for $p >1$.}
\begin{solution}
\begin{align*}
g(x) = e^{-\alpha |x|^p} 
\end{align*}
Since, $g$ is not differentiable for $x = 0$, we are going analyse concavity on two intervals: $[-1, 0)$ and $(0, 1]$.
\begin{itemize}
\item $x \in [-1, 0)$
\begin{align*}
g(x) & = e^{-\alpha (-x)^p} \\
g'(x) & = \alpha p (-x)^{p - 1} e^{-\alpha (-x)^p}  \\
g''(x) & = - \alpha p (p - 1) (-x)^{p - 2} e^{-\alpha (-x)^p} + \alpha p (-x)^{p - 1} \alpha p (-x)^{p - 1} e^{-\alpha (-x)^p} \\
\end{align*}
$\Rightarrow$
\begin{align*}
g''(x) & \leq 0 \\
- \alpha p (p - 1) (-x)^{p - 2} e^{-\alpha (-x)^p} + \alpha p (-x)^{p - 1} \alpha p (-x)^{p - 1} e^{-\alpha (-x)^p} & \leq 0 \\
- (p - 1) (-x)^{-1} +  (-x)^{p - 1} \alpha p & \leq 0 \\
(-x)^{p - 1} \alpha p & \leq \frac{p - 1}{-x}  \\
\alpha & \leq \frac{p - 1}{p (-x) (-x)^{p - 1} }  \\
\alpha & \leq \frac{p - 1}{p (-x)^{p} }  \\
\end{align*}
$\Rightarrow$
\begin{align*}
\alpha & = \min_{x \in [-1, 0)} \frac{p - 1}{p (-x)^{p} }  \\
\alpha & = \frac{p - 1}{p}
\end{align*}
\item $x \in (0, 1]$
\begin{align*}
g(x) & = e^{-\alpha x^p} \\
g'(x) & = -\alpha p x^{p - 1} e^{-\alpha x^p}  \\
g''(x) & = - \alpha p (p - 1) x^{p - 2} e^{-\alpha x^p} + \alpha p x^{p - 1} \alpha p x^{p - 1} e^{-\alpha x^p} \\
\end{align*}
$\Rightarrow$
\begin{align*}
g''(x) & \leq 0 \\
- \alpha p (p - 1) x^{p - 2} e^{-\alpha x^p} + \alpha p x^{p - 1} \alpha p x^{p - 1} e^{-\alpha x^p} & \leq 0 \\
- (p - 1) x^{-1} + x^{p - 1} \alpha p & \leq 0 \\
x^{p - 1} \alpha p & \leq \frac{p - 1}{x} \\
\alpha & \leq \frac{p - 1}{p x x^{p - 1}} \\
\alpha & \leq \frac{p - 1}{p x^{p}} \\
\end{align*}
$\Rightarrow$
\begin{align*}
\alpha & = \min_{x \in (0, 1]} \frac{p - 1}{p x^{p} }  \\
\alpha & = \frac{p - 1}{p}
\end{align*}
\end{itemize}
We can conclude that $g$ is $\frac{p - 1}{p}$-exp-concave on intervals $[-1, 0)$ and $(0, 1]$. Since $g$ is continuous function on $[-1 ,1]$, it is $\frac{p - 1}{p}$-exp-concave on whole $[-1, 1]$.
\end{solution}
\end{subquestion}

\end{question}

% 4th question
\begin{question}{}

\begin{subquestion}{ Let $f(w) = g( \langle w, x \rangle )$ for some fixed $x$. Show that $f$ is $\alpha$-exp-concave when $g$ is $\alpha$-exp-concave.}
\begin{solution}
\end{solution}
\end{subquestion}

\begin{subquestion}{Let $f(w, y) = g( \langle w, x \rangle, y)$ for some fixed $x$. Show that $f$ is $\eta$-mixable when $g$ is $\eta$-mixable.}
\begin{solution}
\end{solution}
\end{subquestion}

\end{question}

\bibliographystyle{plain}
\bibliography{references}
\end{document}



















