\documentclass{article}
\usepackage[utf8]{inputenc}

\title{MLT Homework 3}
\author{Bas Haver}

\usepackage{natbib}
\usepackage{graphicx}

\usepackage{amsmath}
\usepackage{amsfonts}
\usepackage{amssymb}
\usepackage{bbm}
\usepackage{mathtools}

\usepackage{url}

\DeclarePairedDelimiter\ceil{\lceil}{\rceil}
\DeclarePairedDelimiter\floor{\lfloor}{\rfloor}

\newcounter{counterquestion}
\newenvironment{question}[1]
{
\stepcounter{counterquestion}
\section*{Question \thecounterquestion}
\emph{#1} 
} 
{
}

\newcounter{countersubquestion}[counterquestion]
\newenvironment{subquestion}[1]
{
\stepcounter{countersubquestion}
\subsection*{Subquestion \thecounterquestion .\thecountersubquestion}
\emph{#1} 
} 
{
}

\newenvironment{solution}
{
\subsubsection*{Solution}
} 
{
}


\begin{document}
We will construct a sequence in $\Sigma ^+$ to be able to apply Fatou's Lemma. Since we know $|f_n| \leq g_n$ for all $n\in \mathbb{N}$ and $f_n \to f$ and $g_n \to g$, we have $$|f_n-f|\leq g_n +g$$Therefore we can conclude $g_n + g -|f_n-f| \geq 0$ and in $\Sigma ^+$. Applying fatou's lemma now gives us $$\liminf _{n \to \infty } \mu (g_n+g-|f_n-f|) \geq \mu (\liminf _{n \to \infty } (g_n + g - |f_n - f| )).$$
The RHS equals 2$\mu (g)$, since both $f$ and $g$ converge pointwise. The LHS is equal to $2\mu (g) - \limsup _{n\to \infty }\mu (|f_n-f|)$. By assumption we have $\lim _{n \to \infty} \mu (g_n)=\mu (g)$. Putting it together we obtain $$0\geq \limsup _{n \to \infty } \mu (|f_n - f|)$$
\maketitle


\end{document}